Allow values in (some) unstamped paths
To capture the full pDOT (per #146), we're going to use non-variable values in
some unstamped paths, the ones that we'll use to model type members. This (WIP)
PR generalizes unstamped syntax to prepare for that, by adding an extra
parameter to `is_unstamped`.

theories/Dot/stamping/unstampedness_binding.v
@@ -9,25 +9,25 @@ Implicit Types
          (T: ty) (v: vl) (e: tm) (p: path) (d: dm) (ds: dms) (vs: vls)
          (Γ : ctx) (g: stys) (n: nat).
 
-Definition is_unstamped_sub n m s :=
-  ∀ i, i < n → is_unstamped_vl m (s i).
-Notation is_unstamped_ren n m r := (is_unstamped_sub n m (ren r)).
+Definition is_unstamped_sub n m b s :=
+  ∀ i, i < n → is_unstamped_vl m b (s i).
+Notation is_unstamped_ren n m b r := (is_unstamped_sub n m b (ren r)).
 
 Lemma is_unstamped_nclosed_mut:
-  (∀ t i,
-    is_unstamped_tm i t →
+  (∀ t i b,
+    is_unstamped_tm i b t →
     nclosed t i) ∧
-  (∀ v i,
-    is_unstamped_vl i v →
+  (∀ v i b,
+    is_unstamped_vl i b v →
     nclosed_vl v i) ∧
-  (∀ d i,
-    is_unstamped_dm i d →
+  (∀ d i b,
+    is_unstamped_dm i b d →
     nclosed d i) ∧
-  (∀ p i,
-    is_unstamped_path i p →
+  (∀ p i b,
+    is_unstamped_path i b p →
     nclosed p i) ∧
-  (∀ T i,
-    is_unstamped_ty i T →
+  (∀ T i b,
+    is_unstamped_ty i b T →
     nclosed T i).
 Proof.
   apply syntax_mut_ind; intros; with_is_unstamped inverse => //; ev;
@@ -41,91 +41,91 @@ Proof.
     decompose_Forall; case_match; subst. eauto.
 Qed.
 
-Lemma is_unstamped_nclosed_tm e n: is_unstamped_tm n e → nclosed e n.
+Lemma is_unstamped_nclosed_tm e n b: is_unstamped_tm n b e → nclosed e n.
 Proof. apply is_unstamped_nclosed_mut. Qed.
-Lemma is_unstamped_nclosed_vl v n: is_unstamped_vl n v → nclosed_vl v n.
+Lemma is_unstamped_nclosed_vl v n b: is_unstamped_vl n b v → nclosed_vl v n.
 Proof. apply is_unstamped_nclosed_mut. Qed.
-Lemma is_unstamped_nclosed_dm d n: is_unstamped_dm n d → nclosed d n.
+Lemma is_unstamped_nclosed_dm d n b: is_unstamped_dm n b d → nclosed d n.
 Proof. apply is_unstamped_nclosed_mut. Qed.
-Lemma is_unstamped_nclosed_path p n: is_unstamped_path n p → nclosed p n.
+Lemma is_unstamped_nclosed_path p n b: is_unstamped_path n b p → nclosed p n.
 Proof. apply is_unstamped_nclosed_mut. Qed.
-Lemma is_unstamped_nclosed_ty T n: is_unstamped_ty n T → nclosed T n.
+Lemma is_unstamped_nclosed_ty T n b: is_unstamped_ty n b T → nclosed T n.
 Proof. apply is_unstamped_nclosed_mut. Qed.
 
 Hint Resolve is_unstamped_nclosed_tm is_unstamped_nclosed_vl
   is_unstamped_nclosed_dm is_unstamped_nclosed_path
   is_unstamped_nclosed_ty : core.
 
-Lemma is_unstamped_nclosed_σ σ i:
-  is_unstamped_σ i σ →
+Lemma is_unstamped_nclosed_σ σ i b:
+  is_unstamped_σ i b σ →
   nclosed_σ σ i.
 Proof. intros; decompose_Forall. exact: is_unstamped_nclosed_vl. Qed.
 Hint Resolve is_unstamped_nclosed_ty is_unstamped_nclosed_σ : core.
 
-Lemma is_unstamped_nclosed_sub n m ξ :
-  is_unstamped_sub n m ξ → nclosed_sub n m ξ.
+Lemma is_unstamped_nclosed_sub n m b ξ :
+  is_unstamped_sub n m b ξ → nclosed_sub n m ξ.
 Proof. move => Hst i Hle. apply /is_unstamped_nclosed_vl /Hst/Hle. Qed.
 
 Lemma is_unstamped_weaken_mut:
-  (∀ e__s m n,
-      is_unstamped_tm m e__s →
+  (∀ e__s m n b,
+      is_unstamped_tm m b e__s →
       m <= n →
-      is_unstamped_tm n e__s) ∧
-  (∀ v__s m n,
-      is_unstamped_vl m v__s →
+      is_unstamped_tm n b e__s) ∧
+  (∀ v__s m n b,
+      is_unstamped_vl m b v__s →
       m <= n →
-      is_unstamped_vl n v__s) ∧
-  (∀ d__s m n,
-      is_unstamped_dm m d__s →
+      is_unstamped_vl n b v__s) ∧
+  (∀ d__s m n b,
+      is_unstamped_dm m b d__s →
       m <= n →
-      is_unstamped_dm n d__s) ∧
-  (∀ p__s m n,
-      is_unstamped_path m p__s →
+      is_unstamped_dm n b d__s) ∧
+  (∀ p__s m n b,
+      is_unstamped_path m b p__s →
       m <= n →
-      is_unstamped_path n p__s) ∧
-  (∀ T__s m n,
-      is_unstamped_ty m T__s →
+      is_unstamped_path n b p__s) ∧
+  (∀ T__s m n b,
+      is_unstamped_ty m b T__s →
       m <= n →
-      is_unstamped_ty n T__s).
+      is_unstamped_ty n b T__s).
 Proof.
   apply syntax_mut_ind;
     by [intros; with_is_unstamped inverse; econstructor;
       decompose_Forall; eauto with lia].
 Qed.
 
-Lemma is_unstamped_weaken_tm e__s m n:
-  is_unstamped_tm m e__s →
+Lemma is_unstamped_weaken_tm e__s m n b:
+  is_unstamped_tm m b e__s →
   m <= n →
-  is_unstamped_tm n e__s.
+  is_unstamped_tm n b e__s.
 Proof. apply (is_unstamped_weaken_mut). Qed.
-Lemma is_unstamped_weaken_vl v__s m n:
-  is_unstamped_vl m v__s →
+Lemma is_unstamped_weaken_vl v__s m n b:
+  is_unstamped_vl m b v__s →
   m <= n →
-  is_unstamped_vl n v__s.
+  is_unstamped_vl n b v__s.
 Proof. apply (is_unstamped_weaken_mut). Qed.
-Lemma is_unstamped_weaken_dm d__s m n:
-  is_unstamped_dm m d__s →
+Lemma is_unstamped_weaken_dm d__s m n b:
+  is_unstamped_dm m b d__s →
   m <= n →
-  is_unstamped_dm n d__s.
+  is_unstamped_dm n b d__s.
 Proof. apply (is_unstamped_weaken_mut). Qed.
-Lemma is_unstamped_weaken_path p__s m n:
-  is_unstamped_path m p__s →
+Lemma is_unstamped_weaken_path p__s m n b:
+  is_unstamped_path m b p__s →
   m <= n →
-  is_unstamped_path n p__s.
+  is_unstamped_path n b p__s.
 Proof. apply (is_unstamped_weaken_mut). Qed.
-Lemma is_unstamped_weaken_ty T__s m n:
-  is_unstamped_ty m T__s →
+Lemma is_unstamped_weaken_ty T__s m n b:
+  is_unstamped_ty m b T__s →
   m <= n →
-  is_unstamped_ty n T__s.
+  is_unstamped_ty n b T__s.
 Proof. apply (is_unstamped_weaken_mut). Qed.
 
-Lemma is_unstamped_weaken_σ σ m n:
-  is_unstamped_σ m σ →
+Lemma is_unstamped_weaken_σ σ m n b:
+  is_unstamped_σ m b σ →
   m <= n →
-  is_unstamped_σ n σ.
+  is_unstamped_σ n b σ.
 Proof. intros; decompose_Forall. exact: is_unstamped_weaken_vl. Qed.
 
-Lemma is_unstamped_idsσ_ren m n j: j + n <= m → is_unstamped_σ m (idsσ n).|[ren (+j)].
+Lemma is_unstamped_idsσ_ren m n j b: j + n <= m → is_unstamped_σ m b (idsσ n).|[ren (+j)].
 Proof.
   elim: n m j => [//=|n IHn] m j Ijm.
   cbn; rewrite (hren_upn_gen 0 1 j) /= plusnO.
@@ -133,17 +133,17 @@ Proof.
   apply IHn; lia.
 Qed.
 
-Lemma is_unstamped_idsσ m n: n <= m → is_unstamped_σ m (idsσ n).
+Lemma is_unstamped_idsσ m n b: n <= m → is_unstamped_σ m b (idsσ n).
 Proof. pose proof (@is_unstamped_idsσ_ren m n 0) as H. asimpl in H. exact: H. Qed.
 Hint Resolve is_unstamped_idsσ : core.
 
-Lemma is_unstamped_ren_shift n m j:
-  m >= j + n → is_unstamped_ren n m (+j).
+Lemma is_unstamped_ren_shift n m j b:
+  m >= j + n → is_unstamped_ren n m b (+j).
 Proof. constructor => //=; lia. Qed.
 
-Lemma is_unstamped_ren_up n m r:
-  is_unstamped_ren n m r →
-  is_unstamped_ren (S n) (S m) (upren r).
+Lemma is_unstamped_ren_up n m r b:
+  is_unstamped_ren n m b r →
+  is_unstamped_ren (S n) (S m) b (upren r).
 Proof.
   (* rewrite /is_unstamped_ren /is_unstamped_sub /=. *)
   move => Hr [|i] //= Hi; first by constructor => /=; lia.
@@ -155,7 +155,7 @@ Hint Resolve is_unstamped_ren_up is_unstamped_ren_shift : core.
 
 From D.Dot Require Import closed_subst.
 
-Lemma is_unstamped_nclosed_ren i j r: is_unstamped_ren i j r → nclosed_ren i j r.
+Lemma is_unstamped_nclosed_ren i j r b: is_unstamped_ren i j b r → nclosed_ren i j r.
 Proof.
   move => /= Hr x Hx. specialize (Hr x Hx); inverse Hr. exact: nclosed_vl_ids.
 Qed.
@@ -165,43 +165,56 @@ Lemma is_unstamped_ren_var v r:
   ∃ x : var, rename r v = var_vl x.
 Proof. naive_solver. Qed.
 
+Lemma is_unstamped_var_intype i j b :
+  is_unstamped_vl i b (ids j) → is_unstamped_vl i InType (ids j).
+Proof. inversion 1; by constructor. Qed.
+Lemma is_unstamped_ren_intype i j b r :
+  is_unstamped_ren i j b r → is_unstamped_ren i j InType r.
+Proof. intros Hu ?**. by eapply is_unstamped_var_intype, Hu. Qed.
+
+Hint Extern 0 (forall_traversal_tm _ _ _) => cbn : core.
+Hint Extern 0 (forall_traversal_vl _ _ _) => cbn : core.
+Hint Extern 0 (forall_traversal_dm _ _ _) => cbn : core.
+Hint Extern 0 (forall_traversal_path _ _ _) => cbn : core.
+Hint Extern 0 (forall_traversal_ty _ _ _) => cbn : core.
+
 Lemma is_unstamped_ren_mut:
-  (∀ t r i j,
-    is_unstamped_ren i j r →
-    is_unstamped_tm i t →
-    is_unstamped_tm j (rename r t)) ∧
-  (∀ v r i j,
-    is_unstamped_ren i j r →
-    is_unstamped_vl i v →
-    is_unstamped_vl j (rename r v)) ∧
-  (∀ d r i j,
-    is_unstamped_ren i j r →
-    is_unstamped_dm i d →
-    is_unstamped_dm j (rename r d)) ∧
-  (∀ p r i j,
-    is_unstamped_ren i j r →
-    is_unstamped_path i p →
-    is_unstamped_path j (rename r p)) ∧
-  (∀ T r i j,
-    is_unstamped_ren i j r →
-    is_unstamped_ty i T →
-    is_unstamped_ty j (rename r T)).
+  (∀ t r i j b,
+    is_unstamped_ren i j b r →
+    is_unstamped_tm i b t →
+    is_unstamped_tm j b (rename r t)) ∧
+  (∀ v r i j b,
+    is_unstamped_ren i j b r →
+    is_unstamped_vl i b v →
+    is_unstamped_vl j b (rename r v)) ∧
+  (∀ d r i j b,
+    is_unstamped_ren i j b r →
+    is_unstamped_dm i b d →
+    is_unstamped_dm j b (rename r d)) ∧
+  (∀ p r i j b,
+    is_unstamped_ren i j b r →
+    is_unstamped_path i b p →
+    is_unstamped_path j b (rename r p)) ∧
+  (∀ T r i j b,
+    is_unstamped_ren i j b r →
+    is_unstamped_ty i b T →
+    is_unstamped_ty j b (rename r T)).
 Proof.
   apply syntax_mut_ind; intros; with_is_unstamped ltac:(fun H => inversion_clear H);
-    cbn in *; try by [|eauto using is_unstamped_ren_var].
+    cbn in *; try by [|naive_solver eauto using is_unstamped_ren_var, is_unstamped_ren_intype].
   - constructor; rewrite list_pair_swap_snd_rename Forall_fmap;
       by decompose_Forall; eauto.
 Qed.
 
-Lemma is_unstamped_ren_vl v r i j:
-  is_unstamped_ren i j r →
-  is_unstamped_vl i v →
-  is_unstamped_vl j (rename r v).
+Lemma is_unstamped_ren_vl v r i j b:
+  is_unstamped_ren i j b r →
+  is_unstamped_vl i b v →
+  is_unstamped_vl j b (rename r v).
 Proof. apply is_unstamped_ren_mut. Qed.
 
-Lemma is_unstamped_sub_up n m s:
-  is_unstamped_sub n m s →
-  is_unstamped_sub (S n) (S m) (up s).
+Lemma is_unstamped_sub_up n m s b:
+  is_unstamped_sub n m b s →
+  is_unstamped_sub (S n) (S m) b (up s).
 Proof.
   move => Hs [|i] Hi //=. by constructor => /=; lia.
   eapply is_unstamped_ren_vl; eauto with lia.
@@ -226,8 +239,8 @@ Abort. *)
 Lemma is_unstamped_sub_mut:
   (∀ t s i j,
     is_unstamped_sub i j s →
-    is_unstamped_tm i t →
-    is_unstamped_tm j t.|[s]) ∧
+    is_unstamped_tm i b t →
+    is_unstamped_tm j b t.|[s]) ∧
   (∀ v s i j,
     is_unstamped_sub i j s →
     is_unstamped_vl i v →
@@ -275,17 +288,17 @@ Proof.
   intros; rewrite Forall_fmap. decompose_Forall. exact: is_unstamped_sub_vl.
 Qed. *)
 
-Lemma is_unstamped_vl_ids i j: i < j → is_unstamped_vl j (ids i).
+Lemma is_unstamped_vl_ids i j b: i < j → is_unstamped_vl j b (ids i).
 Proof. rewrite /ids /ids_vl; by constructor. Qed.
 Hint Resolve is_unstamped_vl_ids : core.
 
-Lemma is_unstamped_sub_stail i j v sb:
-  is_unstamped_sub (S i) j (v .: sb) →
-  is_unstamped_sub i j sb.
+Lemma is_unstamped_sub_stail i j v sb b:
+  is_unstamped_sub (S i) j b (v .: sb) →
+  is_unstamped_sub i j b sb.
 Proof. move => Hs k Hle. apply (Hs (S k)), lt_n_S, Hle. Qed.
 
-Lemma is_unstamped_sub_equiv {σ i} :
-  is_unstamped_σ i σ ↔ is_unstamped_sub (length σ) i (to_subst σ).
+Lemma is_unstamped_sub_equiv {σ i b} :
+  is_unstamped_σ i b σ ↔ is_unstamped_sub (length σ) i b (to_subst σ).
 Proof.
   split; elim: σ => [//| /= v σ IHσ] Hcl/=.
   - by move => ??; lia.
@@ -296,34 +309,34 @@ Qed.
 Hint Resolve -> is_unstamped_sub_equiv : core.
 
 
-Lemma is_unstamped_sub_single n v:
-  is_unstamped_vl n v →
-  is_unstamped_sub (S n) n (v .: ids).
+Lemma is_unstamped_sub_single n v b:
+  is_unstamped_vl n b v →
+  is_unstamped_sub (S n) n b (v .: ids).
 Proof. move => Hv [|i] Hin /=; eauto with lia. Qed.
 
-Lemma is_unstamped_sub_ren_ty T r i j:
-  is_unstamped_ren i j r →
-  is_unstamped_ty i T → is_unstamped_ty j T.|[ren r].
+Lemma is_unstamped_sub_ren_ty T r i j b:
+  is_unstamped_ren i j b r →
+  is_unstamped_ty i b T → is_unstamped_ty j b T.|[ren r].
 Proof. rewrite -ty_rename_Lemma. apply is_unstamped_ren_mut. Qed.
 
-Lemma is_unstamped_sub_ren_path p r i j:
-  is_unstamped_ren i j r →
-  is_unstamped_path i p → is_unstamped_path j p.|[ren r].
+Lemma is_unstamped_sub_ren_path p r i j b:
+  is_unstamped_ren i j b r →
+  is_unstamped_path i b p → is_unstamped_path j b p.|[ren r].
 Proof. rewrite -path_rename_Lemma. apply is_unstamped_ren_mut. Qed.
 
 
-Lemma is_unstamped_ren1 i : is_unstamped_ren i (S i) (+1).
+Lemma is_unstamped_ren1 i b : is_unstamped_ren i (S i) b (+1).
 Proof. apply is_unstamped_ren_shift; lia. Qed.
 Hint Resolve is_unstamped_ren1 : core.
 
-Lemma is_unstamped_ren1_ty i T:
-  is_unstamped_ty i T ->
-  is_unstamped_ty (S i) (T.|[ren (+1)]).
+Lemma is_unstamped_ren1_ty i T b:
+  is_unstamped_ty i b T ->
+  is_unstamped_ty (S i) b (T.|[ren (+1)]).
 Proof. exact: is_unstamped_sub_ren_ty. Qed.
 
-Lemma is_unstamped_ren1_path i p:
-  is_unstamped_path i p ->
-  is_unstamped_path (S i) (shift p).
+Lemma is_unstamped_ren1_path i p b:
+  is_unstamped_path i b p ->
+  is_unstamped_path (S i) b (shift p).
 Proof. exact: is_unstamped_sub_ren_path. Qed.
 
 
@@ -335,29 +348,29 @@ Proof. intros [x ?]; destruct v; simplify_eq; eauto. Qed.
 Lemma is_unstamped_sub_rev_mut:
   (∀ e i,
     nclosed e i →
-    ∀ s j,
-    is_unstamped_tm j (e.|[s]) →
-    is_unstamped_tm i e) ∧
+    ∀ s j b,
+    is_unstamped_tm j b (e.|[s]) →
+    is_unstamped_tm i b e) ∧
   (∀ v i,
     nclosed_vl v i →
-    ∀ s j,
-    is_unstamped_vl j (v.[s]) →
-    is_unstamped_vl i v) ∧
+    ∀ s j b,
+    is_unstamped_vl j b (v.[s]) →
+    is_unstamped_vl i b v) ∧
   (∀ d i,
     nclosed d i →
-    ∀ s j,
-    is_unstamped_dm j (d.|[s]) →
-    is_unstamped_dm i d) ∧
+    ∀ s j b,
+    is_unstamped_dm j b (d.|[s]) →
+    is_unstamped_dm i b d) ∧
   (∀ p i,
     nclosed p i →
-    ∀ s j,
-    is_unstamped_path j (p.|[s]) →
-    is_unstamped_path i p) ∧
+    ∀ s j b,
+    is_unstamped_path j b (p.|[s]) →
+    is_unstamped_path i b p) ∧
   (∀ T i,
     nclosed T i →
-    ∀ s j,
-    is_unstamped_ty j (T.|[s]) →
-    is_unstamped_ty i T).
+    ∀ s j b,
+    is_unstamped_ty j b (T.|[s]) →
+    is_unstamped_ty i b T).
 Proof.
   apply nclosed_syntax_mut_ind => /=; intros;
     with_is_unstamped ltac:(fun H => try nosplit (inverse H)); ev;
@@ -368,28 +381,29 @@ Proof.
     constructor => /=.
     rewrite ->?@Forall_fmap in *.
     decompose_Forall. destruct x; cbn in *. eauto.
+  - constructor; naive_solver eauto using is_unstamped_sub_rev_var.
 Qed.
 
-Lemma is_unstamped_sub_rev_vl v s i j:
+Lemma is_unstamped_sub_rev_vl v s i j b:
   nclosed_vl v i →
-  is_unstamped_vl j (v.[s]) →
-  is_unstamped_vl i v.
+  is_unstamped_vl j b (v.[s]) →
+  is_unstamped_vl i b v.
 Proof. unmut_lemma is_unstamped_sub_rev_mut. Qed.
-Lemma is_unstamped_sub_rev_ty T s i j:
+Lemma is_unstamped_sub_rev_ty T s i j b:
   nclosed T i →
-  is_unstamped_ty j (T.|[s]) →
-  is_unstamped_ty i T.
+  is_unstamped_ty j b (T.|[s]) →
+  is_unstamped_ty i b T.
 Proof. unmut_lemma is_unstamped_sub_rev_mut. Qed.
 
-Lemma is_unstamped_sub_one_rev i T v:
+Lemma is_unstamped_sub_one_rev i b T v:
   nclosed T (S i) →
-  is_unstamped_ty i (T.|[v/]) →
-  is_unstamped_ty (S i) T.
+  is_unstamped_ty i b (T.|[v/]) →
+  is_unstamped_ty (S i) b T.
 Proof. intros; by eapply is_unstamped_sub_rev_ty. Qed.
 
-Lemma is_unstamped_ren_ty i T:
-  is_unstamped_ty i T <->
-  is_unstamped_ty (S i) (T.|[ren (+1)]).
+Lemma is_unstamped_ren_ty i b T:
+  is_unstamped_ty i b T <->
+  is_unstamped_ty (S i) b (T.|[ren (+1)]).
 Proof.
   split; first exact: is_unstamped_ren1_ty.
   intros Hu.
