theories/Dot/stamping/traversals.v
@@ -11,6 +11,7 @@ Module Trav1.
 Record Traversal {travStateT: Type} :=
   {
     upS: travStateT → travStateT;
+    intoTypeS: travStateT → travStateT;
     varP: travStateT → nat → Prop;
     dtysynP: travStateT → ty → Prop;
     dtysemP: travStateT → vls → stamp → ty → travStateT → Prop;
@@ -108,10 +109,10 @@ Section fold.
       forall_traversal_ty ts T2 →
       forall_traversal_ty ts (TTMem l T1 T2)
   | trav_TSel ts p l:
-      forall_traversal_path ts p →
+      forall_traversal_path (trav.(intoTypeS) ts) p →
       forall_traversal_ty ts (TSel p l)
   | trav_TSing ts p:
-      forall_traversal_path ts p →
+      forall_traversal_path (trav.(intoTypeS) ts) p →
       forall_traversal_ty ts (TSing p)
   | trav_TPrim ts b: forall_traversal_ty ts (TPrim b)
     .
