theories/Dot/typing/typing_unstamped_derived.v
@@ -5,10 +5,10 @@ From D.Dot Require Import unstampedness_binding.
 From D.Dot Require Import path_repl_lemmas typingStamping.
 Import DBNotation.
 
-Lemma is_unstamped_pvar i n : i < n → is_unstamped_path n (pv (var_vl i)).
-Proof. eauto. Qed.
+Lemma is_unstamped_pvar i n b : i < n → is_unstamped_path n b (pv (var_vl i)).
+Proof. eauto 6. Qed.
 Hint Resolve is_unstamped_pvar : core.
-Lemma is_unstamped_pvars i n l : i < n → is_unstamped_ty n (pv (var_vl i) @; l).
+Lemma is_unstamped_pvars i n l b : i < n → is_unstamped_ty n b (pv (var_vl i) @; l).
 Proof. eauto. Qed.
 Hint Resolve is_unstamped_pvars : core.
 Lemma unstamped_subject_closed {Γ e T}
@@ -35,7 +35,7 @@ Ltac tcrush := repeat first [ eassumption | reflexivity | typconstructor | stcru
 Lemma Appv_typed Γ e1 x2 T1 T2:
   Γ u⊢ₜ e1: TAll T1 T2 →
   Γ u⊢ₜ tv (var_vl x2) : T1 →
-  is_unstamped_ty (S (length Γ)) T2 →
+  is_unstamped_ty' (S (length Γ)) T2 →
   (*────────────────────────────────────────────────────────────*)
   Γ u⊢ₜ tapp e1 (tv (var_vl x2)) : T2.|[(var_vl x2)/].
 Proof.
@@ -47,7 +47,7 @@ Qed.
 Lemma TMuE_typed Γ x T:
   Γ u⊢ₜ tv (var_vl x): TMu T →
   (*──────────────────────*)
-  is_unstamped_ty (S (length Γ)) T →
+  is_unstamped_ty' (S (length Γ)) T →
   Γ u⊢ₜ tv (var_vl x): T.|[(var_vl x)/].
 Proof.
   move => + Hu. rewrite -(psubst_subst_agree_ty (n := S (length Γ))) // => Hx.
@@ -57,7 +57,7 @@ Qed.
 Lemma TMuI_typed Γ x T:
   Γ u⊢ₜ tv (var_vl x): T.|[(var_vl x)/] →
   (*──────────────────────*)
-  is_unstamped_ty (S (length Γ)) T →
+  is_unstamped_ty' (S (length Γ)) T →
   Γ u⊢ₜ tv (var_vl x): TMu T.
 Proof.
   move => + Hu. rewrite -(psubst_subst_agree_ty (n := S (length Γ))) // => Hx.
@@ -70,8 +70,8 @@ Ltac tcrush ::=
   typconstructor | stcrush ].
 
 Lemma is_unstamped_TLater_n i {n T}:
-  is_unstamped_ty n T →
-  is_unstamped_ty n (iterate TLater i T).
+  is_unstamped_ty' n T →
+  is_unstamped_ty' n (iterate TLater i T).
 Proof. elim: i => [|//i IHi]; rewrite ?iterate_0 ?iterate_S //; auto. Qed.
 
 Ltac wtcrush := repeat first [ fast_done | typconstructor | stcrush ] ; try solve [
@@ -168,7 +168,7 @@ Ltac varsub := (eapply Var0_typed_sub || eapply Var_typed_sub); first done.
 Lemma Appv_typed' T2 {Γ e1 x2 T1 T3} :
   Γ u⊢ₜ e1: TAll T1 T2 →                        Γ u⊢ₜ tv (ids x2) : T1 →
   T3 = T2.|[ids x2/] →
-  is_unstamped_ty (S (length Γ)) T2 →
+  is_unstamped_ty' (S (length Γ)) T2 →
   (*────────────────────────────────────────────────────────────*)
   Γ u⊢ₜ tapp e1 (tv (ids x2)) : T3.
 Proof. intros; subst; exact: Appv_typed. Qed.
@@ -176,21 +176,21 @@ Proof. intros; subst; exact: Appv_typed. Qed.
 Lemma TMuE_typed' Γ x T1 T2:
   Γ u⊢ₜ tv (ids x): μ T1 →
   T2 = T1.|[ids x/] →
-  is_unstamped_ty (S (length Γ)) T1 →
+  is_unstamped_ty' (S (length Γ)) T1 →
   (*──────────────────────*)
   Γ u⊢ₜ tv (ids x): T2.
 Proof. intros; subst; tcrush. Qed.
 
 Lemma Sub_later_shift {Γ T1 T2 i j}
-  (Hs1: is_unstamped_ty (length Γ) T1)
-  (Hs2: is_unstamped_ty (length Γ) T2)
+  (Hs1: is_unstamped_ty' (length Γ) T1)
+  (Hs2: is_unstamped_ty' (length Γ) T2)
   (Hsub: Γ u⊢ₜ T1, S i <: T2, S j):
   Γ u⊢ₜ TLater T1, i <: TLater T2, j.
 Proof. by asideLaters. Qed.
 
 Lemma Sub_later_shift_inv {Γ T1 T2 i j}
-  (Hs1: is_unstamped_ty (length Γ) T1)
-  (Hs2: is_unstamped_ty (length Γ) T2)
+  (Hs1: is_unstamped_ty' (length Γ) T1)
+  (Hs2: is_unstamped_ty' (length Γ) T2)
   (Hsub: Γ u⊢ₜ TLater T1, i <: TLater T2, j):
   Γ u⊢ₜ T1, S i <: T2, S j.
 Proof.
@@ -199,14 +199,14 @@ Proof.
 Qed.
 
 Lemma LSel_stp' Γ U {p l L i}:
-  is_unstamped_ty (length Γ) L →
+  is_unstamped_ty' (length Γ) L →
   Γ u⊢ₚ p : TTMem l L U, i →
   Γ u⊢ₜ L, i <: TSel p l, i.
 Proof. intros; ettrans; last exact: (@LSel_stp _ p); tcrush. Qed.
 
 (* Worse than dty_typed, but shown in the paper. *)
 Lemma dty_typed_intermediate Γ T V l L U:
-  is_unstamped_ty (S (length Γ)) T →
+  is_unstamped_ty' (S (length Γ)) T →
   TLater V :: Γ u⊢ₜ L, 0 <: T, 0 →
   TLater V :: Γ u⊢ₜ T, 0 <: U, 0 →
   Γ |d V u⊢{ l := dtysyn T } : TTMem l L U.
@@ -214,7 +214,7 @@ Proof. intros; apply dty_typed; tcrush. Qed.
 
 (** * Manipulating laters, basics. *)
 
-Lemma AddIJ_stp {Γ T} i j (Hst: is_unstamped_ty (length Γ) T) :
+Lemma AddIJ_stp {Γ T} i j (Hst: is_unstamped_ty' (length Γ) T) :
   Γ u⊢ₜ T, j <: T, i + j.
 Proof.
   elim: i => [|n IHn]; first tcrush.
@@ -222,7 +222,7 @@ Proof.
   ettrans; [exact: TAddLater_stp | tcrush].
 Qed.
 
-Lemma AddI_stp Γ T i (Hst: is_unstamped_ty (length Γ) T) :
+Lemma AddI_stp Γ T i (Hst: is_unstamped_ty' (length Γ) T) :
   Γ u⊢ₜ T, 0 <: T, i.
 Proof. rewrite -(plusnO i). by apply (AddIJ_stp i 0). Qed.
 
@@ -239,7 +239,7 @@ Qed.
 Lemma Let_typed Γ t u T U :
   Γ u⊢ₜ t : T →
   T.|[ren (+1)] :: Γ u⊢ₜ u : U.|[ren (+1)] →
-  is_unstamped_ty (length Γ) T →
+  is_unstamped_ty' (length Γ) T →
   Γ u⊢ₜ lett t u : U.
 Proof. move => Ht Hu HsT. apply /App_typed /Ht /Lam_typed /Hu /HsT. Qed.
 
@@ -255,26 +255,26 @@ Proof. intros; eapply AddIB_stp, SelU_stp; tcrush. Qed.
 
 (* These rules from storeless typing must be encoded somehow via variables. *)
 (* Lemma packTV_LB T n Γ i :
-  is_unstamped_ty n T →
+  is_unstamped_ty' n T →
   n <= length Γ →
   Γ u⊢ₜ ▶: T, i <: (pv (packTV T) @; "A"), i.
 Proof. intros; apply /val_LB /packTV_typed'. Qed. *)
 
 (* Lemma packTV_UB T n Γ i :
-  is_unstamped_ty n T →
+  is_unstamped_ty' n T →
   n <= length Γ →
   Γ u⊢ₜ (pv (packTV T) @; "A"), i <: ▶: T, i.
 Proof. intros; by apply /val_UB /packTV_typed'. Qed. *)
 
 Lemma Dty_typed Γ T V l:
-  is_unstamped_ty (S (length Γ)) T →
+  is_unstamped_ty' (S (length Γ)) T →
   Γ |d V u⊢{ l := dtysyn T } : TTMem l T T.
 Proof. intros. tcrush. Qed.
 
 (* We can derive rules Bind1 and Bind2 (the latter only conjectured) from
   "Type Soundness for Dependent Object Types (DOT)", Rompf and Amin, OOPSLA '16. *)
 Lemma Bind1 Γ T1 T2 i:
-  is_unstamped_ty (S (length Γ)) T1 → is_unstamped_ty (length Γ) T2 →
+  is_unstamped_ty' (S (length Γ)) T1 → is_unstamped_ty' (length Γ) T2 →
   iterate TLater i T1 :: Γ u⊢ₜ T1, i <: T2.|[ren (+1)], i →
   Γ u⊢ₜ μ T1, i <: T2, i.
 Proof.
@@ -284,7 +284,7 @@ Proof.
 Qed.
 
 Lemma Bind2 Γ T1 T2 i:
-  is_unstamped_ty (length Γ) T1 → is_unstamped_ty (S (length Γ)) T2 →
+  is_unstamped_ty' (length Γ) T1 → is_unstamped_ty' (S (length Γ)) T2 →
   iterate TLater i T1.|[ren (+1)] :: Γ u⊢ₜ T1.|[ren (+1)], i <: T2, i →
   Γ u⊢ₜ T1, i <: μ T2, i.
 Proof.
@@ -293,13 +293,13 @@ Proof.
 Qed.
 
 Lemma Bind1' Γ T1 T2:
-  is_unstamped_ty (S (length Γ)) T1 → is_unstamped_ty (length Γ) T2 →
+  is_unstamped_ty' (S (length Γ)) T1 → is_unstamped_ty' (length Γ) T2 →
   T1 :: Γ u⊢ₜ T1, 0 <: T2.|[ren (+1)], 0 →
   Γ u⊢ₜ μ T1, 0 <: T2, 0.
 Proof. intros; exact: Bind1. Qed.
 
 Lemma Bind2' Γ T1 T2:
-  is_unstamped_ty (length Γ) T1 → is_unstamped_ty (S (length Γ)) T2 →
+  is_unstamped_ty' (length Γ) T1 → is_unstamped_ty' (S (length Γ)) T2 →
   T1.|[ren (+1)] :: Γ u⊢ₜ T1.|[ren (+1)], 0 <: T2, 0 →
   Γ u⊢ₜ T1, 0 <: μ T2, 0.
 Proof. intros; exact: Bind2. Qed.
@@ -308,8 +308,8 @@ Ltac mltcrush := tcrush; try ((apply Bind1' || apply Bind1); tcrush); repeat loo
 
 (* Simplified package introduction, for talk. *)
 Lemma BindSpec Γ (L T U : ty):
-  is_unstamped_ty (S (length Γ)) T →
-  is_unstamped_ty (S (length Γ)) L → is_unstamped_ty (S (length Γ)) U →
+  is_unstamped_ty' (S (length Γ)) T →
+  is_unstamped_ty' (S (length Γ)) L → is_unstamped_ty' (S (length Γ)) U →
   {@ type "A" >: T <: T }%ty :: Γ u⊢ₜ L, 0 <: T, 0 →
   {@ type "A" >: T <: T }%ty :: Γ u⊢ₜ T, 0 <: U, 0 →
   Γ u⊢ₜ tv (ν {@ type "A" = T }) : μ {@ type "A" >: L <: U }.
@@ -329,7 +329,7 @@ Proof.
 Qed.
 
 Lemma psingleton_sym_typed Γ p q i:
-  is_unstamped_path (length Γ) q →
+  is_unstamped_path' (length Γ) q →
   Γ u⊢ₚ p : TSing q, i →
   Γ u⊢ₚ q : TSing p, i.
 Proof.
@@ -341,9 +341,9 @@ Qed.
 
 Lemma PSub_singleton_stp_inv {Γ i p q T1 T2}:
   T1 ~Tp[ p := q ]* T2 →
-  is_unstamped_ty (length Γ) T1 →
-  is_unstamped_ty (length Γ) T2 →
-  is_unstamped_path (length Γ) p →
+  is_unstamped_ty' (length Γ) T1 →
+  is_unstamped_ty' (length Γ) T2 →
+  is_unstamped_path' (length Γ) p →
   Γ u⊢ₚ q : TSing p, i →
   Γ u⊢ₜ T1, i <: T2, i.
 Proof. intros. by eapply PSub_singleton_stp, psingleton_sym_typed. Qed.
@@ -359,14 +359,14 @@ Qed.
 
 Lemma Mu_stp' {Γ T T' i}:
   T' = shift T →
-  is_unstamped_ty (length Γ) T →
+  is_unstamped_ty' (length Γ) T →
   Γ u⊢ₜ μ T', i <: T, i.
 Proof. intros; subst. auto. Qed.
 
 Lemma dvabs_sub_typed {Γ} V T1 T2 e l L:
   shift T1 :: V :: Γ u⊢ₜ e : T2 →
   TLater V :: Γ u⊢ₜ TAll T1 T2, 0 <: L, 0 →
-  is_unstamped_ty (S (length Γ)) T1 →
+  is_unstamped_ty' (S (length Γ)) T1 →
   Γ |d V u⊢{ l := dvl (vabs e) } : TVMem l L.
 Proof.
   intros He Hsub Hs.
@@ -379,7 +379,7 @@ Qed.
 Definition packTV l T := (ν {@ type l = shift T }).
 
 Lemma packTV_typed' T n Γ l :
-  is_unstamped_ty n T →
+  is_unstamped_ty' n T →
   n <= length Γ →
   Γ u⊢ₜ tv (packTV l T) : typeEq l T.
 Proof.
@@ -390,7 +390,7 @@ Proof.
 Qed.
 
 Lemma packTV_typed T Γ l :
-  is_unstamped_ty (length Γ) T →
+  is_unstamped_ty' (length Γ) T →
   Γ u⊢ₜ tv (packTV l T) : typeEq l T.
 Proof. intros; exact: packTV_typed'. Qed.
 
@@ -403,8 +403,8 @@ Lemma tyApp_typed Γ T U V t l :
     for ML and Scala: that is, producing a type [V] that does not refer to
     variables bound by let in the expression. *)
   (∀ L, typeEq l T.|[ren (+2)] :: L :: Γ u⊢ₜ U.|[up (ren (+1))], 0 <: V.|[ren (+2)], 0) →
-  is_unstamped_ty (length Γ) T →
-  is_unstamped_ty (S (length Γ)) U →
+  is_unstamped_ty' (length Γ) T →
+  is_unstamped_ty' (S (length Γ)) U →
   Γ u⊢ₜ tyApp t l T : V.
 Proof.
   move => Ht Hsub HuT1 HuU1.
@@ -415,7 +415,7 @@ Proof.
   apply /Subs_typed_nocoerce /Hsub.
 
   eapply Appv_typed'; first var.
-  have HuT3 : is_unstamped_ty (S (S (length Γ))) (shiftN 2 T)
+  have HuT3 : is_unstamped_ty' (S (S (length Γ))) (shiftN 2 T)
     by rewrite hrenS; wtcrush.
   varsub; tcrush; rewrite !hsubst_comp; f_equal. autosubst.
   asimpl.
@@ -427,7 +427,7 @@ Qed.
 
  *)
 Lemma TLaterRN_stp Γ T i j:
-  is_unstamped_ty (length Γ) T →
+  is_unstamped_ty' (length Γ) T →
   Γ u⊢ₜ T, j + i <: iterate TLater j T, i.
 Proof.
   elim: j T => /= [|j IHj] T HuT; rewrite ?iterate_0 ?iterate_Sr /=; tcrush.
@@ -437,7 +437,7 @@ Proof.
 Qed.
 
 Lemma TLaterLN_stp {Γ T} i j :
-  is_unstamped_ty (length Γ) T →
+  is_unstamped_ty' (length Γ) T →
   Γ u⊢ₜ iterate TLater j T, i <: T, j + i.
 Proof.
   elim: j T => /= [|j IHj] T HuT; rewrite ?iterate_0 ?iterate_Sr /=; tcrush.
@@ -450,8 +450,8 @@ Qed.
 Lemma dropLaters Γ e T U i:
   Γ u⊢ₜ e : T →
   Γ u⊢ₜ T, 0 <: iterate TLater i U, 0 →
-  is_unstamped_ty (length Γ) T →
-  is_unstamped_ty (length Γ) U →
+  is_unstamped_ty' (length Γ) T →
+  is_unstamped_ty' (length Γ) U →
   Γ u⊢ₜ iterate tskip i e : TAnd T U.
 Proof.
   intros HeT Hsub HuT HuU.
@@ -471,8 +471,8 @@ Lemma deLaterSingV0 {Γ} p i e T U:
   Γ u⊢ₚ p : TSing p, 0 →
   shift (TSing p) :: Γ u⊢ₜ shift (TSing p), 0 <: iterate TLater i T, 0 →
   TAnd (TSing (shiftN 2 p)) (shift T) :: TSing (shift p) :: Γ u⊢ₜ e : shiftN 2 U →
-  is_unstamped_ty (length Γ) T →
-  is_unstamped_path (length Γ) p →
+  is_unstamped_ty' (length Γ) T →
+  is_unstamped_path' (length Γ) p →
   Γ u⊢ₜ deLater (path2tm p) i e : U.
 Proof.
   intros HpT1 Hsub HeU HuT Hup.
@@ -487,9 +487,9 @@ Lemma deLaterSingV1 {Γ} p i e T1 T2 U:
   shift (TAnd (TSing p) T1) :: Γ u⊢ₜ shift T1, 0 <: iterate TLater i T2, 0 →
   TAnd (TAnd (TSing (shiftN 2 p)) (shiftN 2 T1)) (shift T2) ::
     TAnd (TSing (shift p)) (shift T1) :: Γ u⊢ₜ e : shiftN 2 U →
-  is_unstamped_ty (length Γ) T1 →
-  is_unstamped_ty (length Γ) T2 →
-  is_unstamped_path (length Γ) p →
+  is_unstamped_ty' (length Γ) T1 →
+  is_unstamped_ty' (length Γ) T2 →
+  is_unstamped_path' (length Γ) p →
   Γ u⊢ₜ deLater (path2tm p) i e : U.
 Proof.
   intros HpT1 Hsub HeU HuT1 HuT2 Hup.
@@ -504,8 +504,8 @@ Lemma deLaterSing {Γ} p i e T1 U:
   Γ u⊢ₚ p : iterate TLater i T1, 0 →
   TAnd (TSing (shiftN 2 p)) (shiftN 2 T1) ::
     TAnd (TSing (shift p)) (iterate TLater i (shift T1)) :: Γ u⊢ₜ e : shiftN 2 U →
-  is_unstamped_ty (length Γ) T1 →
-  is_unstamped_path (length Γ) p →
+  is_unstamped_ty' (length Γ) T1 →
+  is_unstamped_path' (length Γ) p →
   Γ u⊢ₜ deLater (path2tm p) i e : U.
 Proof.
   intros HpT1 HeU HuT1 Hup.
@@ -519,27 +519,27 @@ Proof.
 Qed.
 
 Lemma selfIntersect Γ T U i j:
-  is_unstamped_ty (length Γ) T →
+  is_unstamped_ty' (length Γ) T →
   Γ u⊢ₜ T, i <: U, j + i →
   Γ u⊢ₜ T, i <: TAnd U T, j + i .
 Proof. intros; tcrush. exact: AddIJ_stp. Qed.
 
 Lemma TDistr_TLater_And_stp Γ T1 T2 i :
-  is_unstamped_ty (length Γ) T1 →
-  is_unstamped_ty (length Γ) T2 →
+  is_unstamped_ty' (length Γ) T1 →
+  is_unstamped_ty' (length Γ) T2 →
   Γ u⊢ₜ TAnd (TLater T1) (TLater T2), i <: TLater (TAnd T1 T2), i.
 Proof. intros; asideLaters; tcrush; [lThis|lNext]. Qed.
 
 (** Inverse of [TDistr_TLater_And_stp]. *)
 Lemma TDistr_TLater_And_stp_inv Γ T1 T2 i :
-  is_unstamped_ty (length Γ) T1 →
-  is_unstamped_ty (length Γ) T2 →
+  is_unstamped_ty' (length Γ) T1 →
+  is_unstamped_ty' (length Γ) T2 →
   Γ u⊢ₜ TLater (TAnd T1 T2), i <: TAnd (TLater T1) (TLater T2), i.
 Proof. intros; tcrush. Qed.
 
 Lemma TDistr_TLater_Or_stp Γ T1 T2 i :
-  is_unstamped_ty (length Γ) T1 →
-  is_unstamped_ty (length Γ) T2 →
+  is_unstamped_ty' (length Γ) T1 →
+  is_unstamped_ty' (length Γ) T2 →
   Γ u⊢ₜ TLater (TOr T1 T2), i <: TOr (TLater T1) (TLater T2), i.
 Proof.
   intros; asideLaters; typconstructor; ettrans;
@@ -548,40 +548,40 @@ Qed.
 
 (** Inverse of [TDistr_TLater_Or_stp]. *)
 Lemma TDistr_TLater_Or_stp_inv Γ T1 T2 i :
-  is_unstamped_ty (length Γ) T1 →
-  is_unstamped_ty (length Γ) T2 →
+  is_unstamped_ty' (length Γ) T1 →
+  is_unstamped_ty' (length Γ) T2 →
   Γ u⊢ₜ TOr (TLater T1) (TLater T2), i <: TLater (TOr T1 T2), i.
 Proof. intros; tcrush. Qed.
 
 (** TLater swaps with TMu, part 1. *)
 Lemma TDistr_TLater_Mu_stp Γ T i :
-  is_unstamped_ty (S (length Γ)) T →
+  is_unstamped_ty' (S (length Γ)) T →
   Γ u⊢ₜ TLater (TMu T), i <: TMu (TLater T), i.
 Proof. intros; asideLaters; tcrush. Qed.
 
 (** TLater swaps with TMu, part 2. *)
 Lemma TDistr_TLater_Mu_stp_inv Γ T i :
-  is_unstamped_ty (S (length Γ)) T →
+  is_unstamped_ty' (S (length Γ)) T →
   Γ u⊢ₜ TMu (TLater T), i <: TLater (TMu T), i.
 Proof. intros; asideLaters; tcrush. Qed.
 
 (** Show that [singleton_Mu_[12]] and [p_mu_[ie]_typed] are interderivable. *)
 Lemma singleton_Mu_1 {Γ p T i} :
   Γ u⊢ₚ p : TMu T, i →
-  is_unstamped_ty (S (length Γ)) T →
+  is_unstamped_ty' (S (length Γ)) T →
   Γ u⊢ₜ TSing p, i <: T .Tp[ p /], i.
 Proof. intros Hp Hu; apply PSelf_singleton_stp, (p_mu_e_typed Hu Hp). Qed.
 
 Lemma singleton_Mu_2 {Γ p T i} :
   Γ u⊢ₚ p : T .Tp[ p /], i →
-  is_unstamped_ty (S (length Γ)) T →
+  is_unstamped_ty' (S (length Γ)) T →
   Γ u⊢ₜ TSing p, i <: TMu T, i.
 Proof. intros Hp Hu; apply PSelf_singleton_stp, (p_mu_i_typed Hu Hp). Qed.
 
 (* Avoid automation, to ensure we don't use [p_mu_e_typed] to show them. *)
 Lemma p_mu_e_typed' {Γ T p i} :
   Γ u⊢ₚ p : TMu T, i →
-  is_unstamped_ty (S (length Γ)) T →
+  is_unstamped_ty' (S (length Γ)) T →
   Γ u⊢ₚ p : T .Tp[ p /], i.
 Proof.
   intros Hp Hu. eapply p_subs_typed', (psingleton_refl_typed Hp).
@@ -590,7 +590,7 @@ Qed.
 
 Lemma p_mu_i_typed' {Γ T p i} :
   Γ u⊢ₚ p : T .Tp[ p /], i →
-  is_unstamped_ty (S (length Γ)) T →
+  is_unstamped_ty' (S (length Γ)) T →
   Γ u⊢ₚ p : TMu T, i.
 Proof.
   intros Hp Hu. eapply p_subs_typed', (psingleton_refl_typed Hp).
@@ -616,7 +616,7 @@ On the other hand, this derived rule handles the substitution in [T2] directly.
 Lemma singleton_Mu_dotty1 {Γ p i T1' T2} :
   Γ u⊢ₜ T1', i <: T2 .Tp[ p /], i →
   Γ u⊢ₚ p : T1', i →
-  is_unstamped_ty (S (length Γ)) T2 →
+  is_unstamped_ty' (S (length Γ)) T2 →
   Γ u⊢ₜ TSing p, i <: TMu T2, i.
 Proof.
   intros Hsub Hp Hu.
@@ -629,7 +629,7 @@ Definition anfBind t := lett t (tv x0).
 Lemma AnfBind_typed Γ t (T U: ty) :
   Γ u⊢ₜ t : T →
   shift T :: Γ u⊢ₜ tv x0 : shift U →
-  is_unstamped_ty (length Γ) T →
+  is_unstamped_ty' (length Γ) T →
   Γ u⊢ₜ anfBind t : U.
 Proof. intros; eapply Let_typed; eauto. Qed.
 
